coq/Corps/Types.v
@@ -2,19 +2,20 @@ Require Import EqBool.
 Require Import Syntax.
 Require Import RelationClasses.
 Require Import Lia.
+Require Import Coq.Program.Equality.
 
 Section CorpsTypes.
   Context {PName : Type} `{EqBool PName}.
 
+  #[local] Notation Ctxt := (@Ctxt PName).
   #[local] Notation type := (type PName).
   #[local] Notation expr := (expr PName).
   #[local] Notation mod := (mod PName).
   #[local] Definition ptm := @proc_to_mod PName.
   Coercion ptm : PName >-> mod.
+  Context {CanSend CanUp CanDown : mod -> mod -> Prop}.
   
   Section TypeSystem.
-
-    Context {CanSend CanUp CanDown : mod -> mod -> Prop}.
 
     Inductive Typed : Ctxt -> expr -> type -> Prop :=
     | VarTyping {Γ : Ctxt} {n : nat} {τ : type} (m : mod) (pf1 : vars Γ n = (m, τ)) (pf2 : locks Γ n = m)
@@ -55,10 +56,11 @@ Section CorpsTypes.
         (pf1 : Typed Γ e1 (ArrT τ1 τ2))
         (pf2 : Typed Γ e2 τ1)
       : Typed Γ (appE e1 e2) τ2
-    | SendTyping {Γ : Ctxt} {p q : PName} {Δ : FiniteCtxt} {e : expr} {τ : type}
+    | SendTyping {Γ Γ' : Ctxt} {p q : PName} {Δ : FiniteCtxt} {e : expr} {τ : type}
         (pf : Typed (addFiniteCtxt (add_lock Γ p) Δ) e τ)
         (cs : CanSend (cons (all_locks Γ) p) (cons (all_locks Γ) q))
-      : Typed (addFiniteCtxt (add_lock Γ q) Δ) (send e p Δ q) τ
+        (eqv : ctxt_equiv Γ' (addFiniteCtxt (add_lock Γ q) Δ))
+      : Typed Γ' (send e p Δ q) τ
     | UpTyping {Γ : Ctxt} {p : PName} {Δ : FiniteCtxt} {e : expr} {τ : type}
         (pf : Typed (addFiniteCtxt Γ Δ) e τ)
         (cu : CanUp (all_locks Γ) (cons (all_locks Γ) p))
@@ -69,10 +71,173 @@ Section CorpsTypes.
       : Typed (addFiniteCtxt Γ Δ) (down e p Δ) τ
     .
 
-    
-    
+    Theorem add_lock_ext : forall (Γ Δ : Ctxt) m, ctxt_equiv Γ Δ -> ctxt_equiv (add_lock Γ m) (add_lock Δ m).
+    Proof using.
+      intros Γ Δ m eqv; destruct eqv as [vars_eq [locks_eq all_locks_eq]]; split; [| split]; cbn;
+        auto.
+      - intros x; destruct x; cbn; auto.
+        all: rewrite locks_eq; reflexivity.
+      - rewrite all_locks_eq; reflexivity.
+    Qed.
 
-  End TypeSystem.  
+    Theorem add_var_ext : forall (Γ Δ : Ctxt) m τ, ctxt_equiv Γ Δ -> ctxt_equiv (add_var Γ m τ) (add_var Δ m τ).
+    Proof using.
+      intros Γ Δ m τ [vars_eq [locks_eq all_locks_eq]]; split; [| split]; cbn.
+      1,2 : intro x; destruct x.
+      all: auto.
+    Qed.
+
+    Theorem add_finite_ctxt_ext : forall Γ Δ E,
+        ctxt_equiv Γ Δ -> ctxt_equiv (addFiniteCtxt Γ E) (@addFiniteCtxt PName Δ E).
+    Proof using.
+      intros Γ Δ E; revert Γ Δ; induction E; intros Γ Δ eqv; cbn; auto;
+        apply IHE; [apply add_var_ext; auto | apply add_lock_ext; auto].
+    Qed.
+
+    Theorem type_ext : forall (Γ Δ : Ctxt) (e : expr) (τ : type),
+        Typed Γ e τ -> (ctxt_equiv Γ Δ) -> Typed Δ e τ.
+    Proof using.
+      intros Γ Δ e τ typd; revert Δ; induction typd; try (rename Δ into Γ'); intros Δ' eqv';
+        pose proof (proj1 eqv') as vars_eq;
+        pose proof (proj1 (proj2 eqv')) as locks_eq;
+        pose proof (proj2 (proj2 eqv')) as all_locks_eq;
+        repeat match goal with
+          | [ H : vars ?Γ ?n = ?x, H' : forall x, vars ?Γ x = vars ?Δ x |- _ ] =>
+              lazymatch goal with
+              | [ _ : vars Δ n = x |- _ ] => fail
+              | _ => assert (vars Δ n = x) by (rewrite <- H'; exact H)
+              end
+          | [ H : locks ?Γ ?n = ?x, H' : forall x, locks ?Γ x = locks ?Δ x |- _ ] =>
+              lazymatch goal with
+              | [ _ : locks Δ n = x |- _ ] => fail
+              | _ => assert (locks Δ n = x) by (rewrite <- H'; exact H)
+              end
+          | [ IH : forall Δ, ctxt_equiv (add_lock ?Γ ?m) Δ -> Typed Δ ?e ?τ, H : ctxt_equiv ?Γ ?Δ |- _ ] =>
+              lazymatch goal with
+              | [ _ : Typed (add_lock Δ m) e τ |- _ ] => fail
+              | _ => pose proof (IH (add_lock Δ m) (add_lock_ext Γ Δ m H))
+              end
+          | [ IH : forall Δ, ctxt_equiv (add_var ?Γ ?m ?τ') Δ -> Typed Δ ?e ?τ, H : ctxt_equiv ?Γ ?Δ |- _ ] =>
+              lazymatch goal with
+              | [ _ : Typed (add_var Δ m τ') e τ |- _ ] => fail
+              | _ => pose proof (IH (add_var Δ m τ') (add_var_ext Γ Δ m τ' H))
+              end
+          | [ IH : forall Δ, ctxt_equiv (addFiniteCtxt ?Γ ?E) Δ -> Typed Δ ?e ?τ, H : ctxt_equiv ?Γ ?Δ |- _ ] =>
+              lazymatch goal with
+              | [ _ : Typed (addFiniteCtxt Δ E) e τ |- _ ] => fail
+              | _ => pose proof (IH (addFiniteCtxt Δ E) (add_finite_ctxt_ext Γ Δ E H))
+              end
+          end;
+        try (econstructor; eauto; fail).
+      - apply @SendTyping with (Γ := Γ); auto.
+        transitivity Γ'; auto. symmetry; assumption.
+      - admit.
+      - admit.
+    Admitted.
+
+    Definition ctxt_ren (Γ : Ctxt) (ξ : renaming) (mono : forall n m, n <= m -> PrefixOf (locks Γ (ξ n)) (locks Γ (ξ m))): Ctxt :=
+      {|
+        vars n := vars Γ (ξ n);
+        locks n := locks Γ (ξ n);
+        all_locks := all_locks Γ;
+        locks_mono n m lt := mono n m lt;
+        locks_bound n := locks_bound Γ (ξ n);
+      |}.
+
+    Lemma weakening : forall (Γ Δ : Ctxt) (e : expr) (ξ : renaming) (τ : type) mono,
+        ctxt_equiv (ctxt_ren Γ ξ mono) Δ ->
+        Typed Δ e τ -> Typed Γ (ren e ξ) τ.
+    Proof using.
+      intros Γ Δ e ξ τ mono eqv typ; revert Γ ξ mono eqv; induction typ;
+        intros Γ'' ξ mono [vars_eqv [locks_eqv al_eqv]]; cbn.
+      all: try (econstructor; eauto; fail).
+      - apply VarTyping with (m := m).  rewrite <- pf1; rewrite <- vars_eqv; cbn; reflexivity.
+        rewrite <- pf2; rewrite <- locks_eqv; cbn; reflexivity.
+      - apply AtTyping. eapply IHtyp. Unshelve.
+        2: { intros n m H0; cbn; apply mod_app_mono_l; apply mono; auto. }
+        split; [|split].
+        -- intro x; cbn. rewrite <- vars_eqv. cbn. reflexivity.
+        -- intro x; cbn. rewrite <- locks_eqv. cbn. reflexivity.
+        --
+      Admitted.
+
+
+  End TypeSystem.
+
+  Section Substitution.
+
+    Definition TypedSubst (Γ : Ctxt) (σ : substitution) (Δ : Ctxt) :=
+      forall x, match PrefixOfT_dec (locks Γ x) (fst (vars Γ x)) with
+           | Some pfxt => Typed (add_lock Δ (remove_PrefixT pfxt)) (σ x) (snd (vars Γ x))
+           | None => True
+           end.
+      
+    Lemma substup_typed : forall Γ Δ σ τ,
+        TypedSubst Γ σ Δ -> TypedSubst (add_var Γ base τ) (substup σ) (add_var Δ base τ).
+    Proof using.
+      intros Γ Δ σ τ typd; unfold TypedSubst in *; intros x; destruct x; cbn.
+      - econstructor; eauto; reflexivity.
+      - specialize (typd x); destruct (PrefixOfT_dec (locks Γ x) (fst (vars Γ x))); [|exact I].
+        eapply weakening with (Δ := add_lock Δ (remove_PrefixT p)); auto.
+        Unshelve.
+        -- split; [|split].
+           1,2: intro n.
+           all: cbn; reflexivity.
+        -- intros n m H0; apply locks_mono; lia.
+    Qed.
+    
+    Theorem subst_typed : forall Γ Δ e σ τ, Typed Γ e τ -> TypedSubst Γ σ Δ -> Typed Δ (subst e σ) τ.
+    Proof using.
+      intros Γ Δ e σ τ typed; revert Δ σ; induction typed; try (rename σ into τ');
+        intros Γ'' σ typeds; cbn.
+      all: try (econstructor; eauto; fail).
+      - unfold TypedSubst in typeds; specialize (typeds n).
+        rewrite pf1 in typeds; rewrite pf2 in typeds; cbn in typeds.
+        destruct (PrefixOfT_dec m m) eqn:eq.
+        2: { exfalso; destruct (Prefix2PrefixT (PO_refl m)) as [pfxt eq'];
+             rewrite eq' in eq; inversion eq. }
+        assert (p = POT_refl m) by apply UIprefixT; subst. cbn in typeds.
+        apply type_ext with (Γ := add_lock Γ'' base); auto.
+        split; [| split]; cbn; auto; [intro x|]; apply mod_base_app.
+      - apply AtTyping.
+        apply IHtyped.
+        unfold TypedSubst; unfold TypedSubst in typeds.
+        intro x; specialize (typeds x); cbn.
+        destruct (PrefixOfT_dec (mod_app p (locks Γ x)) (fst (vars Γ x))) as [pfxt |];
+          [| exact I].
+        
+
+                                             
+
+  (* Section Decidability. *)
+
+  (*   Program Fixpoint typedb (Γ : Ctxt) (e : expr) (τ : type) : bool := *)
+  (*     match e with *)
+  (*     | var x => eqb (locks Γ x, τ) (vars Γ x) *)
+  (*     | uu => eqb τ UnitT *)
+  (*     | atE p e => *)
+  (*         match τ with *)
+  (*         | AtT q σ => *)
+  (*             eqb p q && typedb (add_lock Γ p) e σ *)
+  (*         | _ => false *)
+  (*         end *)
+  (*     | letAt p e1 e2 => _ *)
+  (*     | pair e1 e2 => _ *)
+  (*     | pi1 e => _ *)
+  (*     | pi2 e => _ *)
+  (*     | inl e => _ *)
+  (*     | inr e => _ *)
+  (*     | caseE e1 e2 e3 => _ *)
+  (*     | efql e => _ *)
+  (*     | lam t e => _ *)
+  (*     | appE e1 e2 => _ *)
+  (*     | send e p Δ q => _ *)
+  (*     | up e p Δ => _ *)
+  (*     | down e p Δ => _ *)
+  (*     end. *)
+  (*   Next Obligation. *)
+
+  (* End Decidability. *)
   
 End CorpsTypes.
 
